Disjoint.v
@@ -15,9 +15,11 @@ Parameter loop_splits : forall `{redCFG}, Lab -> Lab -> list (Lab * Lab * Lab).
 
 (* remove branch from splits, we can use the assumed global branch function to get varsets back*)
 Definition pl_split `{redCFG} (qh qe q1 q2 br : Lab) :=
-  (exists π ϕ, CPath br qh (π >: q1 :>: br)
-          /\ CPath br qe (ϕ >: q2 :>: br)
-          /\ q1 <> q2
+  (exists π ϕ, CPath br qh (π :>: br)
+          /\ CPath br qe (ϕ :>: br)
+          /\ q1 = ne_back π
+          /\ q2 = ne_back ϕ
+          /\ q1 <> q2 (* if π = single or φ = single, then this is not implied by the next condition *)
           /\ Disjoint (tl π) (tl ϕ)).
 
 Parameter path_splits_spec (* unused *): forall `{redCFG} p q1 q2 br,
@@ -26,6 +28,7 @@ Parameter path_splits_spec (* unused *): forall `{redCFG} p q1 q2 br,
 
 Parameter loop_splits_spec (* unused *): forall `{redCFG} qh qe q1 q2 br,
     loop_contains qh br /\ (* otherwise some splits would be considered as loop splits *)
+    exited qh qe /\
     pl_split qh qe q1 q2 br <->
     (br, q1, q2) ∈ loop_splits qh qe.
 
@@ -84,30 +87,7 @@ Qed.
 Local Arguments deq_loop {_ _ _ _} _.
 Local Arguments depth {_ _ _ _} _.
 Local Arguments exited {_ _ _ _} _.
-(*Lemma head_exits_head_inv (* unused *)`(C : redCFG) (h : Lab)
-  : loop_head C h <->loop_head (head_exits_CFG C) h.
-Admitted.
-Lemma head_exits_exited_inv `(C : redCFG) (h p : Lab)
-  : exited C h p <-> exited (head_exits_CFG C) h p.
-Admitted.*)
-Lemma head_exits_deq_loop_inv1 `(C : redCFG) (h p q : Lab)
-  : deq_loop C p q -> deq_loop (head_exits_CFG C h) p q.
-Admitted.
-(*
-Lemma head_exits_depth_inv (* unused *)`(C : redCFG) (p : Lab)
-  : depth C p = depth (head_exits_CFG C) p.
-Admitted.
-*)
-(*
-Lemma no_strictly_containing_loop_impl_top_level:
-  forall (Lab : finType) (edge : Lab -> Lab -> bool) (root : Lab) (a_edge : Lab -> Lab -> bool)
-    (C : redCFG edge root a_edge) (p : Lab),
-    (forall h' : Lab, loop_contains h' p -> h' = p) ->
-    implode_nodes C p.
-Proof.
-  intros.
-Admitted.
-*)
+
 Definition thrice (A B : Type) (f : A -> B) (xyz : A*A*A) : B*B*B
   := match xyz with (x,y,z) => (f x, f y, f z) end.
 
@@ -180,6 +160,7 @@ Parameter splits'_spec (* unused *)
   : forall `{redCFG} h e sp, sp ∈ splits' h e
                         <-> sp ∈ loop_splits__imp h e
                           \/ exists br q q', (br,q,q') ∈ loop_splits__imp h e
+                                       /\ exited br q /\ exited br q'
                                        /\ (sp ∈ splits' br q
                                           \/ sp ∈ splits' br q').
 
@@ -197,6 +178,7 @@ Parameter splits_spec
                         \/ (exists h, (* lsplits of exited loops: *)
                               exited h p /\ sp ∈ splits' h p)
                         \/ exists br q q',(br,q,q') ∈ path_splits__imp p
+                                    /\ exited br q /\ exited br q'
                                     (* loop_split of splitting heads *)
                                     /\ (sp ∈ splits' br q
                                        \/ sp ∈ splits' br q').
@@ -254,15 +236,19 @@ Arguments loop_head {_ _ _ _ _}.
 Arguments loop_head_dec {_ _ _ _ _}.
 Arguments get_innermost_loop_strict {_ _ _ _ _}. 
 
-Fixpoint impl_list' `{redCFG} (h : Lab) (l : list Coord) :=
+Fixpoint impl_list' `{redCFG} (r : Lab) (l : list Coord) :=
   match l with
   | nil => nil
-  | (q,j) :: l => if decision ((loop_contains h q \/ exited h q) /\ deq_loop h q)
-                 then (q,j) :: impl_list' h l
-                 else if decision (exists e : Lab, exited q e /\ deq_loop h e)
-                      then (q,tl j) :: impl_list' h l
-                      else impl_list' h l
+  | (q,j) :: l => match decision (deq_loop r q) with
+                 | left H => (impl_of_original' (h:=r) (p:=q) (or_introl H), j) :: impl_list' r l
+                 | right H => match decision (exists e : Lab, exited q e /\ deq_loop r e) with
+                             | left Q => (impl_of_original' (h:=r) (p:=q) (or_intror Q), tl j) :: impl_list' r l
+                             | right Q => impl_list' r l
+                             end
+                 end
   end.
+
+Definition innermost_loop' `{redCFG} (h p : Lab) := (loop_contains h p \/ h = root) /\ deq_loop h p.
 
 Definition get_innermost_loop_strict' `{C : redCFG} p
   := match get_innermost_loop_strict p with
@@ -406,17 +392,86 @@ Proof.
   destructH. eexists;eexists. eapply in_app_or in Hlc. destruct Hlc;eauto.
 Qed.
 
-Lemma lc_implode_in `{redCFG} p q1 q2 h s i j1 j2 k t1 t2
-      (Hpath1 : TPath' ((p,i) :<: (q1,j1) :< t1))
-      (Hpath2 : TPath' ((p,i) :<: (q2,j2) :< t2))
-      (Hlc : last_common ((q1,j1) :: t1) ((q2,j2) :: t2) (s,k))
-      (Hinner : innermost_loop h p)
-      (Hdep : depth p < depth s)
-  : exists h', loop_contains h' s
-          /\ last_common (impl_list' h ((q1,j1) :: t1))
-                        (impl_list' h ((q2,j2) :: t2))
-                        (h', i).
+Lemma impl_list'_tpath `{C:redCFG} p i h t
+      (Hpath : TPath' ((p,i) :< t))
+      (Hp : deq_loop h p)
+  : TPath' (C:=local_impl_CFG C h) ((impl_of_original' (or_introl Hp),i) :< impl_list' h t).
 Admitted.
+
+Lemma lc_implode_in `{redCFG} p s i k t1 t2
+      (Hpath1 : TPath' ((p,i) :< t1))
+      (Hpath2 : TPath' ((p,i) :< t2))
+      (Hlc : last_common t1 t2 (s,k))
+      (Hdep : depth p < depth s) (*TODO*)
+  : exists h', loop_contains (`h') s
+          /\ last_common (impl_list' p t1) (impl_list' p t2) (h', i).
+Admitted.
+
+Lemma lc_implode_out `{redCFG} p s i k t1 t2
+      (Hpath1 : TPath' ((p,i) :< t1))
+      (Hpath2 : TPath' ((p,i) :< t2))
+      (Hlc : last_common t1 t2 (s,k))
+      (Hdeq : deq_loop p s)
+  : exists s', (`s') = s /\ last_common (impl_list' p t1) (impl_list' p t2) (s',k).
+Admitted.
+
+Lemma lc_cut {A : Type} `{EqDec A eq} (l1 l2 : list A) (a : A)
+      (Hlc : last_common l1 l2 a)
+  : exists l1' l2', last_common (l1' :r: a) (l2' :r: a) a /\ Postfix (l1' :r: a) l1 /\ Postfix (l2' :r: a) l2.
+Proof.
+  unfold last_common in Hlc.
+  destructH.
+  exists l1', l2'. split;eauto.
+  unfold last_common. exists l1', l2'. split_conj;auto.
+  1,2: econstructor.
+Qed.
+
+Lemma lc_same_tags `{C:redCFG} s k l1 l2 t1 t2
+      (Hpost1 : Postfix (l1 :r: (s, k)) t1)
+      (Hpost2 : Postfix (l2 :r: (s, k)) t2)
+      (Hdisj : Disjoint l1 l2)
+      p i
+      (Hpath1 : TPath' ((p, i) :< t1))
+      (Hpath2 : TPath' ((p, i) :< t2))
+      (Heq  : eq_loop p s)
+      (Hdeq : forall q, deq_loop p q)
+  : forall q j, (q,j) ∈ l1 -> j = k.
+Admitted.
+
+Lemma disj_fst {A B : Type} `{EqDec A eq} `{Q:EqDec B eq} (l1 l2 : list (A * B)) k
+      (Hdisj : Disjoint l1 l2)
+      (Hsame1 : forall q j, (q,j) ∈ l1 -> j = k)
+      (Hsame2 : forall q j, (q,j) ∈ l2 -> j = k)
+  : Disjoint (map fst l1) (map fst l2).
+Proof.
+  eapply disjoint2. intros.
+  intro Hneq. 
+  enough ((x,k) = (y,k)).
+  {
+    revert H2. eapply disjoint2.
+    - eapply Hdisj.
+    - eapply in_fst in H0. destructH. replace k with b by eauto. eauto.
+    - eapply in_fst in H1. destructH. replace k with b by eauto. eauto.
+  }
+  f_equal. auto.
+Qed.
+
+Lemma path_splits_in_imp `{C:redCFG} (p : Lab) (s q q' : local_impl_CFG_type C p)
+  : let D := local_impl_CFG C p in
+    let p' := (impl_of_original' (C:=C) (or_introl (deq_loop_refl (C:=C) (l:=p)))) in
+    (`s,`q,`q') ∈ path_splits__imp p
+    <-> (s,q,q') ∈ @path_splits _ _ _ _ D p'.
+Admitted.
+
+Lemma ex_path_splits__imp `{C:redCFG} (p : Lab) (s : local_impl_CFG_type C p)
+  : (exists q q', (s, q, q') ∈ @path_splits _ _ _ _ (local_impl_CFG C p)
+                       (impl_of_original' (C:=C) (or_introl (deq_loop_refl (C:=C) (l:=p)))))
+    -> exists q q', (`s, q, q') ∈ path_splits__imp p.
+Proof.
+  intros.
+  destructH.
+  exists (`q), (`q'). eapply path_splits_in_imp. auto.
+Qed.
 
 Theorem lc_join_split `{redCFG} t1 t2 (p q1 q2 s : Lab) (i j1 j2 k : Tag)
         (* it is important to cons qj's in front of the t's *)
@@ -426,20 +481,76 @@ Theorem lc_join_split `{redCFG} t1 t2 (p q1 q2 s : Lab) (i j1 j2 k : Tag)
         (Hpath2 : TPath' ((p,i) :<: (q2,j2) :< t2))
   : exists qq qq', (s,qq,qq') ∈ splits p.
 Proof.
-  destruct (Nat.lt_trichotomy (depth s) (depth p)) as [Htri|[Htri|Htri]].
-  - exfalso.
-    (* the tag k is shorter than i
-     * some head has to be visited from outside on the way from s to p
-     * this head has the same tag on both traces 0 :: k, contradiction to last_common *)
-    admit.
-  - (* k = i, bc otherwise we would visit the head of p in both traces with the same tag,
+  decide (deq_loop s p) as [Hdeq|Hndeq].
+  decide (deq_loop p s) as [Hdeq'|Hndeq'].
+  - enough (exists qq qq', (s, qq, qq') ∈ path_splits__imp p).
+    { destructH. eexists; eexists. eapply splits_spec. left. eauto. }
+    (* cut last_common such that (s,k) is the back of the list 
+     * eapply lc_implode_out
+     * then use tpath lemma on TPath (s,k) (p,i) t gives us TPath (C:=implCFG) (s,k) (p,i) (impl_list' h t)
+     *)
+    
+    eapply lc_implode_out in Hlc;eauto.
+    destructH.
+    unfold last_common in Hlc1. destructH.
+    specialize (@lc_same_tags _ _ _ _ (local_impl_CFG H p) s' k l1' l2') as Hsame.
+    fold (local_impl_CFG_type H p) in *.
+    specialize (Hsame _ _ Hlc2 Hlc1 Hlc3).
+    replace ((p,i) :<: (q1, j1) :< t1) with ((p,i) :< ((q1,j1) :: t1)) in Hpath1 by (cbn;auto).
+    eapply impl_list'_tpath in Hpath1 as Hpath1'.
+    replace ((p,i) :<: (q2, j2) :< t2) with ((p,i) :< ((q2,j2) :: t2)) in Hpath2 by (cbn;auto).
+    eapply impl_list'_tpath in Hpath2 as Hpath2'.
+    specialize (Hsame _ i Hpath1' Hpath2').
+    Unshelve. 2: { eapply deq_loop_refl. }
+    exploit' Hsame. admit.
+    exploit' Hsame. admit.
+    assert (forall q j, (q,j) ∈ l2' -> j = k) as Hsame' by admit.
+
+    eapply disj_fst in Hlc3;eauto.
+    rewrite <-Hlc0.
+    eapply ex_path_splits__imp. fold (local_impl_CFG_type H p).
+    set (p' := (impl_of_original' (or_introl (deq_loop_refl (l:=p))))) in *.
+    exists (ne_back (p' :< map fst l1')).
+    exists (ne_back (p' :< map fst l2')).
+    eapply path_splits_spec.
+    unfold pl_split.
+    exists (p' :< (map fst l1')), (p' :< (map fst l2')).
+    split_conj;eauto.
+    + eapply path_postfix_path in Hpath1';cycle 1.
+      * simpl_nl. eapply postfix_cons. eapply Hlc2.
+      * simpl_nl' Hpath1'. clear - Hpath1'. admit. (* some path reasoning (easy) *)
+    + admit. (* as above *)
+    + admit. (* Show that p is not in l1' & l2' (possibly difficult) *)
+    + simpl_nl. cbn. auto. 
+  (* this gives disjoint cpaths *)
+    
+    
+      
+    
+    (* k = i, bc otherwise we would visit the head of p in both traces with the same tag,
      * which contradicts Hlc *)
-    replace k with i in * by admit.
-    eapply lc_join_path_split in Hlc;eauto.
-    destructH.
-    eexists; eexists. eapply splits_spec. left. eauto.
-  - eapply lc_implode_in in Htri;cycle 2;eauto. admit.
-    destructH.
+    (* this is not true for p being a head. 
+     * instead I need something that all tags from s to p (excluding p) are equal k to *)
+  - enough (exists br q q' : Lab, (br, q, q') ∈ path_splits__imp p
+                             /\ (exists qq qq', (s, qq, qq') ∈ splits' br q \/ (s, qq, qq') ∈ splits' br q')).
+    { destructH. exists qq, qq'. eapply splits_spec. right. right. repeat eexists.
+      all: admit. (* new goals because of modification to the splits_spec *)
+    }
+(*    eapply lc_implode_in in Htri;cycle 2;eauto.
+    + instantiate (1:=h). admit.
+    + destructH. cbn in Htri1.*)
+    admit.
+  - simpl_dec' Hndeq. simpl_dec' Hndeq. destructH.
+    decide (x = p).
+    + subst. decide (deq_loop p s) as [Hdeq'|Hndeq'].
+      * admit. (* Attention! special case where loop_head p *)
+      * admit. 
+    + exfalso.
+      (* the tag k is shorter than i
+       * some head has to be visited from outside on the way from s to p
+       * this head has the same tag on both traces 0 :: k, contradiction to last_common *)
+      admit.
+      
 Admitted.
 
 
